himpl1

theories/SLFHimpl.v
@@ -11,7 +11,8 @@ License: MIT.
 
 Set Implicit Arguments.
 From TLC Require Import LibCore.
-From Sep Require Import Semantics. 
+From Sep Require Import Semantics.
+
 (* TODO move *)
   Module CoercionsFromStrings.
   Coercion string_to_var (x:string) : var := x.
@@ -23,3 +24,110 @@ From Sep Require Import Semantics.
   Import NotationForVariables NotationForTerms CoercionsFromStrings.
 
 Close Scope fmap_scope.
+
+From Sep Require Import SLFHprop.
+
+
+(* ####################################################### *)
+(** * The chapter in a rush *)
+
+(* ******************************************************* *)
+(** ** Definition of entailment *)
+
+(** The "entailement relationship" [H1 ==> H2] asserts that any
+    heap satisfying [H1] also satisfies [H2]. *)
+
+Definition himpl (H1 H2:hprop) : Prop :=
+  forall (h:heap), H1 h -> H2 h.
+
+Notation "H1 ==> H2" := (himpl H1 H2) (at level 55).
+
+(** [H1 ==> H2] captures the fact that [H1] is a stronger precondition
+    than [H2], in the sense that it is more restrictive.
+
+    It is also useful to describe that a postcondition is stronger than
+    another one, that is, that a postcondition "entails" another one.
+    For that purpose, we introduce [Q1 ===> Q2], which asserts that
+    for any value [v], the heap predicate [Q1 v] entails [Q2 v]. 
+ 
+    Equivalently, [Q1 ===> Q2] holds if for any value [v] and any heap [h],
+    the proposition [Q1 v h] implies [Q2 v h]. *)
+
+Definition qimpl (Q1 Q2:val->hprop) : Prop :=
+  forall (v:val), Q1 v ==> Q2 v.
+
+Notation "Q1 ===> Q2" := (qimpl Q1 Q2) (at level 55).
+
+(** The entailement relation appears in particular in the consequence
+    rule. *)
+
+Lemma rule_conseq : forall t H Q H' Q',
+  triple t H' Q' ->
+  H ==> H' ->
+  Q' ===> Q ->
+  triple t H Q.
+Proof using.
+  introv M WH WQ. rewrite triple_iff_triple_lowlevel in *.
+  unfold triple_lowlevel in *. 
+  intros h1 h2 D P1. lets P1': WH P1.
+  lets M': M D P1'.
+  destruct M' as (v&h1'&h3'&D'&R&HQ).
+  exists v h1' h3'. splits~. applys WQ. auto.
+Qed.
+
+
+
+Parameter himpl_frame_l : forall H2 H1 H1',
+  H1 ==> H1' ->
+  (H1 \* H2) ==> (H1' \* H2).
+
+
+(* ####################################################### *)
+(** * Additional exercises *)
+
+(* ******************************************************* *)
+(** ** Alternative proofs for the consequence rules. *)
+
+(* EX2! (Hoare_conseq) *)
+(** Prove the consequence rule for Hoare triples. *)
+
+Lemma Hoare_conseq : forall t H Q H' Q',
+  Hoare_triple t H' Q' ->
+  H ==> H' ->
+  Q' ===> Q ->
+  Hoare_triple t H Q.
+Proof using.
+(* SOLUTION *)
+  introv M WH WQ. unfold Hoare_triple.
+  intros s Ps. lets Ps': WH Ps.
+  lets M': M Ps'.
+  destruct M' as (v&s'&R&HQ).
+  exists v s'. splits~. applys WQ. auto.
+(* /SOLUTION *)
+Qed.
+
+(* EX2! (rule_conseq) *)
+(** Prove the consequence rule by leveraging the lemma [Hoare_conseq],
+    rather than going through the definition of [triple_lowlevel]. 
+    Hint: apply lemma [Hoare_conseq] with the appropriate arguments,
+    and use lemma [applys himpl_frame_l] to prove the entailments. *)
+
+Lemma rule_conseq' : forall t H Q H' Q',
+  triple t H' Q' ->
+  H ==> H' ->
+  Q' ===> Q ->
+  triple t H Q.
+Proof using.
+(* SOLUTION *)
+  introv M WH WQ. unfold triple. intros H''.
+  applys Hoare_conseq M. 
+  { applys himpl_frame_l. applys WH. }
+  { intros x. applys himpl_frame_l. applys himpl_frame_l. applys WQ. }
+(* /SOLUTION *)
+Qed.
+
+
+
+
+
+From Sep Require Import SepBase.
